Ins_Cycle/Ins_Cycle1.thy
@@ -5,6 +5,10 @@ imports ARM_REF.MMU_ARMv7_Ref
 begin               
 
 
+declare word_extract_def [simp add]
+declare word_bits_def [simp add]
+declare nat_to_bitstring_def [simp add]
+
 
 definition  CP14' :: "CP14"
 where
@@ -415,6 +419,7 @@ where
   SPSR_mon  =            SPSR_mon' ,
   SPSR_svc  =            SPSR_svc',
   SPSR_und  =            SPSR_und',
+  VFPExtension      =     NoVFP,
   exception  =           NoException,
   undefined  =           False,
   (* additional MMU 'b state_scheme *)
@@ -445,6 +450,7 @@ where
   SPSR_mon  =            SPSR_mon' ,
   SPSR_svc  =            SPSR_svc',
   SPSR_und  =            SPSR_und',
+  VFPExtension      =     NoVFP,
   exception  =           NoException,
   undefined  =           False,
   (* additional MMU 'b state_scheme *)
@@ -505,7 +511,7 @@ lemma fetch_ins1:
                             M = True, NMFI = True, RR = True, SW = True, TE = True, U = False, V = False, VE = True, Z = True,
                             sctlr'rst = 1\<rparr>, VBAR = 1\<rparr>,  CPSR = \<lparr>PSR.A = True, C = True, E = False, F = True, GE = 1, I = True, IT = 0, J = False, M = 0x10, N = True, Q = True,
                  T = False, V = True, Z = True, psr'rst = 1\<rparr>,  CurrentCondition = 1, ELR_hyp = 1, Encoding = Encoding_ARM, Extensions = {Extension_Virtualization}, FP = FP', MEM = MEM',
-              REG = Reg_Bank, SPSR_abt = SPSR_abt', SPSR_fiq = SPSR_fiq', SPSR_hyp = SPSR_hyp', SPSR_irq = SPSR_irq', SPSR_mon = SPSR_mon', SPSR_svc = SPSR_svc', SPSR_und = SPSR_und', exception = NoException, undefined = False, TTBR0 = Addr 0, ASID = 1, tlb_set = {pt_walk 1 MEM' (Addr 0) (Addr 0xFC)}\<rparr>)"
+              REG = Reg_Bank, SPSR_abt = SPSR_abt', SPSR_fiq = SPSR_fiq', SPSR_hyp = SPSR_hyp', SPSR_irq = SPSR_irq', SPSR_mon = SPSR_mon', SPSR_svc = SPSR_svc', SPSR_und = SPSR_und',  VFPExtension   =  NoVFP, exception = NoException, undefined = False, TTBR0 = Addr 0, ASID = 1, tlb_set = {pt_walk 1 MEM' (Addr 0) (Addr 0xFC)}\<rparr>)"
   apply (clarsimp simp: Fetch_def CurrentInstrSet_def ISETSTATE_def word_cat_def tlb_state'_def CPSR'_def split:if_split_asm)
   apply ( clarsimp simp:  Reg_Bank_def  MemA_def CurrentModeIsNotUser_def BadMode_def MemA_with_priv_def CP15'_def SCTLR'_def Aligned1_def Align1_def  mmu_read_size_tlb_state_ext_def)
   apply (subgoal_tac "mmu_translate (Addr 0xFC) \<lparr>Architecture = ARMv7_A, CP14 = CP14',  CP15 = \<lparr>HCR = HCR', HSCTLR = HSCTLR', HSR = HSR', MVBAR = 1, NSACR = NSACR', SCR = SCR',
@@ -516,7 +522,7 @@ lemma fetch_ins1:
    T = False, V = True, Z = True, psr'rst = 1\<rparr>,
    CurrentCondition = 1, ELR_hyp = 1, Encoding = Encoding_ARM, Extensions = {Extension_Virtualization}, FP = FP',
    MEM = MEM', REG = Reg_Bank, SPSR_abt = SPSR_abt', SPSR_fiq = SPSR_fiq', SPSR_hyp = SPSR_hyp', SPSR_irq = SPSR_irq',
-   SPSR_mon = SPSR_mon', SPSR_svc = SPSR_svc', SPSR_und = SPSR_und', exception = NoException, undefined = False,
+   SPSR_mon = SPSR_mon', SPSR_svc = SPSR_svc', SPSR_und = SPSR_und',  VFPExtension   =  NoVFP,exception = NoException, undefined = False,
    TTBR0 = Addr 0, ASID = 1, tlb_set = {}\<rparr>
    =  ((Addr 0xFC),   \<lparr>Architecture = ARMv7_A, CP14 = CP14',
    CP15 = \<lparr>HCR = HCR', HSCTLR = HSCTLR', HSR = HSR', MVBAR = 1, NSACR = NSACR', SCR = SCR',
@@ -527,17 +533,17 @@ lemma fetch_ins1:
    T = False, V = True, Z = True, psr'rst = 1\<rparr>,
    CurrentCondition = 1, ELR_hyp = 1, Encoding = Encoding_ARM, Extensions = {Extension_Virtualization}, FP = FP',
    MEM = MEM', REG = Reg_Bank, SPSR_abt = SPSR_abt', SPSR_fiq = SPSR_fiq', SPSR_hyp = SPSR_hyp', SPSR_irq = SPSR_irq',
-   SPSR_mon = SPSR_mon', SPSR_svc = SPSR_svc', SPSR_und = SPSR_und', exception = NoException, undefined = False,
+   SPSR_mon = SPSR_mon', SPSR_svc = SPSR_svc', SPSR_und = SPSR_und',  VFPExtension   =  NoVFP,exception = NoException, undefined = False,
    TTBR0 = Addr 0, ASID = 1, tlb_set = {}\<rparr> \<lparr> tlb_set := {pt_walk 1 MEM' (Addr 0) (Addr 0xFC)}    \<rparr> )")
    prefer 2
    apply (clarsimp simp:  mmu_translate_tlb_state_ext_def tlb_state'_def lookup_def entry_set_def Let_def not_is_fault_MEM')
    apply (clarsimp simp: va_to_pa_def pt_walk_section_MEM' mask_def)
   apply (clarsimp simp: mem_read1_def Let_def mem1_def MEM'_def)
   apply (subgoal_tac "229 = Suc (228) \<and> 130 = Suc (129) \<and> 16 = Suc (15) \<and> 4 = Suc (3)")
-   apply (simp only:"nat_to_bitstring.simps")
-   apply (clarsimp simp:)
+   apply (clarsimp simp:"log2.simps" )
+   apply (clarsimp simp: bitstring_field_def bitstring_shiftr_def fixwidth_def pad_left_def)
   apply simp
-done
+  done
 
 
 
@@ -554,7 +560,7 @@ lemma decode_ins1:
                  T = False, V = True, Z = True, psr'rst = 1\<rparr>,
        CurrentCondition = 1, ELR_hyp = 1, Encoding = Encoding_ARM, Extensions = {Extension_Virtualization}, FP = FP', MEM = MEM',
        REG = Reg_Bank, SPSR_abt = SPSR_abt', SPSR_fiq = SPSR_fiq', SPSR_hyp = SPSR_hyp', SPSR_irq = SPSR_irq', SPSR_mon = SPSR_mon',
-       SPSR_svc = SPSR_svc', SPSR_und = SPSR_und', exception = NoException, undefined = False, TTBR0 = Addr 0, ASID = 1,
+       SPSR_svc = SPSR_svc', SPSR_und = SPSR_und',  VFPExtension   =  NoVFP,exception = NoException, undefined = False, TTBR0 = Addr 0, ASID = 1,
        tlb_set = {pt_walk 1 MEM' (Addr 0) (Addr 0xFC)}\<rparr> = (Store (StoreWord (True, True, False, 1, 2, immediate_form1 4)) , 
        \<lparr>Architecture = ARMv7_A, CP14 = CP14',
        CP15 = \<lparr>HCR = HCR', HSCTLR = HSCTLR', HSR = HSR', MVBAR = 1, NSACR = NSACR', SCR = SCR',
@@ -565,7 +571,7 @@ lemma decode_ins1:
                  T = False, V = True, Z = True, psr'rst = 1\<rparr>,
        CurrentCondition = 0xE, ELR_hyp = 1, Encoding = Encoding_ARM, Extensions = {Extension_Virtualization}, FP = FP', MEM = MEM',
        REG = Reg_Bank, SPSR_abt = SPSR_abt', SPSR_fiq = SPSR_fiq', SPSR_hyp = SPSR_hyp', SPSR_irq = SPSR_irq', SPSR_mon = SPSR_mon',
-       SPSR_svc = SPSR_svc', SPSR_und = SPSR_und', exception = NoException, undefined = False, TTBR0 = Addr 0, ASID = 1,
+       SPSR_svc = SPSR_svc', SPSR_und = SPSR_und',  VFPExtension   =  NoVFP,exception = NoException, undefined = False, TTBR0 = Addr 0, ASID = 1,
        tlb_set = {pt_walk 1 MEM' (Addr 0) (Addr 0xFC)}\<rparr> )"
   apply (clarsimp simp: Decode_def DecodeARM_def Let_def Do_def ConditionPassed_def  CurrentCond_def  mask_def)
 done
@@ -605,7 +611,7 @@ lemma run_ins1:
                            Q = True, T = False, V = True, Z = True, psr'rst = 1\<rparr>,
                  CurrentCondition = 0xE, ELR_hyp = 1, Encoding = Encoding_ARM, Extensions = {Extension_Virtualization}, FP = FP',
                  MEM = MEM', REG = Reg_Bank, SPSR_abt = SPSR_abt', SPSR_fiq = SPSR_fiq', SPSR_hyp = SPSR_hyp', SPSR_irq = SPSR_irq',
-                 SPSR_mon = SPSR_mon', SPSR_svc = SPSR_svc', SPSR_und = SPSR_und', exception = NoException, undefined = False,
+                 SPSR_mon = SPSR_mon', SPSR_svc = SPSR_svc', SPSR_und = SPSR_und', VFPExtension   =  NoVFP, exception = NoException, undefined = False,
                  TTBR0 = Addr 0, ASID = 1, \<dots> = {EntrySection 1 0 (Some 0) 0}\<rparr>)
       1 4 \<noteq>
      Incon ; Run (Store (StoreWord (True, True, False, 1, 2, immediate_form1 4)))
@@ -619,7 +625,7 @@ lemma run_ins1:
                  T = False, V = True, Z = True, psr'rst = 1\<rparr>,
        CurrentCondition = 0xE, ELR_hyp = 1, Encoding = Encoding_ARM, Extensions = {Extension_Virtualization}, FP = FP', MEM = MEM',
        REG = Reg_Bank, SPSR_abt = SPSR_abt', SPSR_fiq = SPSR_fiq', SPSR_hyp = SPSR_hyp', SPSR_irq = SPSR_irq', SPSR_mon = SPSR_mon',
-       SPSR_svc = SPSR_svc', SPSR_und = SPSR_und', exception = NoException, undefined = False, TTBR0 = Addr 0, ASID = 1,
+       SPSR_svc = SPSR_svc', SPSR_und = SPSR_und',  VFPExtension   =  NoVFP,exception = NoException, undefined = False, TTBR0 = Addr 0, ASID = 1,
        tlb_set = {pt_walk 1 MEM' (Addr 0) (Addr 0xFC)}\<rparr>  = (() , s')\<rbrakk> \<Longrightarrow>
     REG s' =  Reg_Bank(RName_PC := 0x100) \<and> MEM s' = MEM'(Addr 4 \<mapsto> 1, Addr 5 \<mapsto> 0, Addr 6 \<mapsto> 0, Addr 7 \<mapsto> 0)"
   apply (clarsimp simp: Run_def dfn'StoreWord_def NullCheckIfThumbEE_def
@@ -637,15 +643,19 @@ lemma run_ins1:
                                 Q = True, T = False, V = True, Z = True, psr'rst = 1\<rparr>,
                       CurrentCondition = 0xE, ELR_hyp = 1, Encoding = Encoding_ARM, Extensions = {Extension_Virtualization}, FP = FP',
                       MEM = MEM', REG = Reg_Bank, SPSR_abt = SPSR_abt', SPSR_fiq = SPSR_fiq', SPSR_hyp = SPSR_hyp',
-                      SPSR_irq = SPSR_irq', SPSR_mon = SPSR_mon', SPSR_svc = SPSR_svc', SPSR_und = SPSR_und', exception = NoException,
+                      SPSR_irq = SPSR_irq', SPSR_mon = SPSR_mon', SPSR_svc = SPSR_svc', SPSR_und = SPSR_und',  VFPExtension   =  NoVFP,exception = NoException,
                       undefined = False, TTBR0 = Addr 0, ASID = 1, \<dots> = {EntrySection 1 0 (Some 0) 0}\<rparr>) 1 4 ")
     apply (clarsimp simp: Let_def is_fault_def  va_to_pa_def pt_walk_section_MEM'_new mask_def write'mem1_def IncPC_def ThisInstrLength_def BranchTo_def Reg_Bank_def)
+    apply (clarsimp simp:"log2.simps" )
+    apply (clarsimp simp: bitstring_field_def bitstring_shiftr_def fixwidth_def pad_left_def)
    apply clarsimp
   apply (subgoal_tac "x3 = EntrySection 1 0 (Some 0) 0")
    apply (clarsimp simp: is_fault_def va_to_pa_def mask_def write'mem1_def IncPC_def ThisInstrLength_def BranchTo_def Reg_Bank_def)
+   apply (clarsimp simp:"log2.simps" )
+   apply (clarsimp simp: bitstring_field_def bitstring_shiftr_def fixwidth_def pad_left_def)
   apply (clarsimp simp: lookup_def entry_set_def split:if_split_asm)
    apply blast+
-done
+  done
 
 
 
